arm atop: Finish proof
Signed-off-by: Kyeongmin Cho <kyeongmin.cho@kaist.ac.kr>

src/axiomatic/SimLocal.v
@@ -498,26 +498,53 @@ Proof.
   refl.
 Qed.
 
-Definition sim_local_vpn ex loc :=
+Definition sim_local_coh_cl ex loc :=
   (⦗ex.(Execution.label_is) (Label.is_accessing_cl loc)⦘ ⨾
-   Execution.po) ∪
+   Execution.po).
 
+Lemma sim_local_coh_cl_step ex loc:
+  sim_local_coh_cl ex loc =
+  (sim_local_coh_cl ex loc ∪
+   (⦗ex.(Execution.label_is) (Label.is_accessing_cl loc)⦘)) ⨾
+  Execution.po_adj.
+Proof.
+  unfold sim_local_coh_cl. rewrite ? (union_seq' Execution.po_adj), ? seq_assoc, ? union_assoc.
+  rewrite Execution.po_po_adj at 1.
+  rewrite (clos_refl_union Execution.po), union_seq, eq_seq.
+  rewrite ? (seq_union' (Execution.po ⨾ Execution.po_adj) Execution.po_adj), ? seq_assoc, ? union_assoc.
+  refl.
+Qed.
+
+Lemma sim_local_coh_cl_spec
+      ex loc1 loc2 eid1 eid2
+      (CL: Loc.cl loc1 loc2):
+  sim_local_coh_cl ex loc1 eid1 eid2 <-> sim_local_coh_cl ex loc2 eid1 eid2.
+Proof.
+  split.
+  - i. inv H. obtac.
+    econs. simtac. econs; eauto.
+    destruct l; ss; eapply Loc.cl_trans; eauto; eapply Loc.cl_sym; ss.
+  - i. inv H. obtac.
+    econs. simtac. econs; eauto.
+    destruct l; ss; eapply Loc.cl_trans; eauto; eapply Loc.cl_sym; ss.
+Qed.
+
+Definition sim_local_vpn ex :=
   (⦗ex.(Execution.label_is) Label.is_access⦘ ⨾
    Execution.po ⨾
    ⦗ex.(Execution.label_is) (Label.is_barrier_c Barrier.is_dmb_dsb_full)⦘ ⨾
    Execution.po).
 
-Lemma sim_local_vpn_step ex loc:
-  sim_local_vpn ex loc =
-  (sim_local_vpn ex loc ∪
-   ((⦗ex.(Execution.label_is) (Label.is_accessing_cl loc)⦘) ∪
-    (⦗ex.(Execution.label_is) Label.is_access⦘ ⨾
+Lemma sim_local_vpn_step ex:
+  sim_local_vpn ex =
+  (sim_local_vpn ex ∪
+   ((⦗ex.(Execution.label_is) Label.is_access⦘ ⨾
      Execution.po ⨾
      ⦗ex.(Execution.label_is) (Label.is_barrier_c Barrier.is_dmb_dsb_full)⦘))) ⨾
   Execution.po_adj.
 Proof.
   unfold sim_local_vpn. rewrite ? (union_seq' Execution.po_adj), ? seq_assoc, ? union_assoc.
-  rewrite Execution.po_po_adj at 1 3.
+  rewrite Execution.po_po_adj at 2.
   rewrite (clos_refl_union Execution.po), union_seq, eq_seq.
   rewrite ? (seq_union' (Execution.po ⨾ Execution.po_adj) Execution.po_adj), ? seq_assoc, ? union_assoc.
   funext. i. funext. i. propext. econs; i.
@@ -532,15 +559,15 @@ Proof.
 Qed.
 
 Definition sim_local_lper ex loc :=
-  (sim_local_vpn ex loc ⨾
-   ⦗ex.(Execution.label_is) (Label.is_flushopting_cl loc)⦘ ⨾
-   Execution.po).
+  ((sim_local_coh_cl ex loc ∪ sim_local_vpn ex) ⨾
+    ⦗ex.(Execution.label_is) (Label.is_flushopting_cl loc)⦘ ⨾
+    Execution.po).
 
 Lemma sim_local_lper_step ex loc:
   sim_local_lper ex loc =
   (sim_local_lper ex loc ∪
-   (sim_local_vpn ex loc ⨾
-    ⦗ex.(Execution.label_is) (Label.is_flushopting_cl loc)⦘)) ⨾
+   ((sim_local_coh_cl ex loc ∪ sim_local_vpn ex) ⨾
+     ⦗ex.(Execution.label_is) (Label.is_flushopting_cl loc)⦘)) ⨾
   Execution.po_adj.
 Proof.
   unfold sim_local_lper. rewrite ? (union_seq' Execution.po_adj), ? seq_assoc, ? union_assoc.
